src/program_proof/session/processClientRequest.v
@@ -80,15 +80,15 @@ Section heap.
       rewrite drop_drop. f_equal.
   Qed.
 
-  Lemma wp_deleteAtIndexMessage (s: Slice.t) (index: w64) (l: list Message.t) (n: nat) :
+  Lemma wp_deleteAtIndexMessage (s: Slice.t) (index: w64) (l: list Message.t) (n: nat) (len_c2s: nat) :
     {{{
         ⌜0 <= uint.nat index < length l⌝ ∗
-        message_slice s l n
+        message_slice s l n len_c2s
     }}}
       deleteAtIndexMessage s #index
     {{{
         (ns: Slice.t), RET slice_val (ns);
-        message_slice ns (coq_deleteAtIndexMessage l (uint.nat index)) n
+        message_slice ns (coq_deleteAtIndexMessage l (uint.nat index)) n len_c2s
     }}}.
   Proof.
     rewrite/ deleteAtIndexMessage. rename s into s1. iIntros (Φ) "[%H_index (%ops1 & H_s1 & H_ops1)] HΦ".
@@ -127,7 +127,7 @@ Section heap.
       iApply big_sepL2_app_equiv. { do 2 rewrite length_take; word. }
       rewrite <- take_drop with (l := ops1) (i := uint.nat index) at 1.
       rewrite <- take_drop with (l := l) (i := uint.nat index) at 1.
-      iAssert (([∗ list] mv;m ∈ take (uint.nat index) ops1;take (uint.nat index) l, ∃ a, ∃ b, is_message mv m n a b) ∗ ([∗ list] mv;m ∈ drop (uint.nat index) ops1;drop (uint.nat index) l, ∃ a, ∃ b, is_message mv m n a b))%I with "[H_ops1]" as "[H_prefix H_suffix]".
+      iAssert (([∗ list] mv;m ∈ take (uint.nat index) ops1;take (uint.nat index) l, ∃ b, is_message mv m n len_c2s b) ∗ ([∗ list] mv;m ∈ drop (uint.nat index) ops1;drop (uint.nat index) l, ∃ b, is_message mv m n len_c2s b))%I with "[H_ops1]" as "[H_prefix H_suffix]".
       { iApply (big_sepL2_app_equiv with "[$H_ops1]"). do 2 rewrite length_take. word. }
       iFrame. destruct (drop (uint.nat index) ops1) as [ | hd tl] eqn: H_obs.
       + iPoseProof (big_sepL2_nil_inv_l with "[$H_suffix]") as "%H_obs'".
